\section{Monomio per binomio}
\begin{equation}
a(b+c)=ab+ac
\end{equation}
\begin{equation}
1(1+2)=11+12
\end{equation}
\section{Binomio per binomio}
\begin{equation}
(a+b)(c+d)=ac+ad+bc+bd
\end{equation}
\begin{equation}
(1+2)(1+2)=11+12+21+22
\end{equation}
\section{Quadrato del binomio}
\begin{equation}
	(a+b)^2=a^2+b^2+2ab
\end{equation}
\begin{equation}
(1+2)^2=1^2+2^2+2(1)(2)
\end{equation}
\section{Quadrato del trinomio}
\begin{equation}
(a+b+c)^2=a^2+b^2+c^2+2ab+2ac+2bc
\end{equation}
\begin{equation}
(1+2+3)^2=1^2+2^2+3^2+2(1)(2)+2(1)(3)+2(2)(3)
\end{equation}
\section{Cubo binomio}
\begin{equation}
(a+b)^3=a^3+b^3+3a^2b+3ab^2
\end{equation}
\begin{equation}
(1+2)^3=1^3+2^3+3(1)^2 2+3(1)2^2
\end{equation}
\section{Differenza di quadrati}
\begin{equation}
(a-b)(a+b)=a^2-b^2
\end{equation}
\begin{equation}
(1-2)(1+2)=1^2-2^2
\end{equation}
